Launchbury.thy
@@ -28,7 +28,7 @@ inductive reds :: "heap \<Rightarrow> exp \<Rightarrow> var list \<Rightarrow> h
 where
   Lambda: "\<Gamma> : (Lam [x]. e) \<Down>\<^bsub>L\<^esub> \<Gamma> : (Lam [x]. e)" 
  | Application: "\<lbrakk> atom y \<sharp> (\<Gamma>,e,x,L,\<Delta>,\<Theta>,z) ; \<Gamma> : e \<Down>\<^bsub>x#L\<^esub> \<Delta> : (Lam [y]. e') ; \<Delta> : e'[y ::= x] \<Down>\<^bsub>L\<^esub> \<Theta> : z\<rbrakk> \<Longrightarrow> \<Gamma> : App e x \<Down>\<^bsub>L\<^esub> \<Theta> : z" 
- | Variable: "\<lbrakk> (x,e) \<in> set \<Gamma>; removeAll (x, e) \<Gamma> : e \<Down>\<^bsub>L\<^esub> \<Delta> : z \<rbrakk> \<Longrightarrow> \<Gamma> : Var x \<Down>\<^bsub>L\<^esub> (x, z) # \<Delta> : z"
+ | Variable: "\<lbrakk> (x,e) \<in> set \<Gamma>; removeAll (x, e) \<Gamma> : e \<Down>\<^bsub>x#L\<^esub> \<Delta> : z \<rbrakk> \<Longrightarrow> \<Gamma> : Var x \<Down>\<^bsub>L\<^esub> (x, z) # \<Delta> : z"
  | Let: "set (bn as) \<sharp>* (\<Gamma>, L) \<Longrightarrow> asToHeap as @ \<Gamma> : body \<Down>\<^bsub>L\<^esub> \<Delta> : z \<Longrightarrow> \<Gamma> : Let as body \<Down>\<^bsub>L\<^esub> \<Delta> : z"
 
 equivariance reds
@@ -88,7 +88,6 @@ next
 case (Variable  x e \<Gamma> L \<Delta> z) thus ?case by (auto simp add: heapVars_def, metis fst_conv imageI)
 next
 case (Let as \<Gamma> L body \<Delta> z)
-  print_facts
   have "x \<notin> heapVars \<Gamma>" by fact moreover
   have "x \<notin> heapVars (asToHeap as)"
     using `set (bn as) \<sharp>* (\<Gamma>, L)` and `x \<in> set L`
